Meta: Axiom.Infinity test

coq/ZF/Meta/Test/Axiom/Infinity.v
@@ -1,50 +1,16 @@
 Require Import Coq.Lists.List.
 Require Import Coq.Strings.String.
 
-Require Import ZF.Meta.Ctx.
-Require Import ZF.Meta.Term.Decl.
-Require Import ZF.Meta.Env.
 Require Import ZF.Meta.Syntax.
 Require Import ZF.Meta.Check.
+Require Import ZF.Meta.Term.CheckDecl.
 Require Import ZF.Meta.Ty.
 
 Import ListNotations.
 
-Definition empty : Decl :=
-  {| paraT := [];
-     resT  := TySet;
-     bodyT := HoleT TySet |}.
+Require Import ZF.Meta.Decl.Axiom.Infinity.
 
-Definition single : Decl :=
-  {| paraT := [TySet];
-     resT  := TySet;
-     bodyT := HoleT TySet |}.
-
-Definition union2 : Decl :=
-  {| paraT := [TySet; TySet];
-     resT  := TySet;
-     bodyT := HoleT TySet |}.
-
-Definition env : Env := Env.fromListT
-  [ ("empty"%string , empty)
-  ; ("single"%string, single)
-  ; ("union2"%string, union2)
-  ].
-
-(* exists a, empty :< a /\ forall x, x :< a -> union2 x (single x) :< a         *)
-Definition Infinity : Term :=
-  Ex VarTySet
-    (And
-      (Elem (IdentT "empty" []) (Var 0))
-      (All VarTySet
-        (Imp
-          (Elem (Var 0) (Var 1))
-          (Elem
-            (IdentT "union2" [Var 0; IdentT "single" [Var 0]])
-            (Var 1))))).
-
-(* The infinity example is a proposition in the local test environment.         *)
-Proposition Check : CheckT env Ctx.empty Infinity TyProp.
+Proposition Infinity : CheckDeclT (Infinity.env) Infinity.
 Proof.
   (* Proof by Hermes + gpt 5.5                                                  *)
   apply CheckEx, CheckAnd.
