coq/ZF/Meta/Decl/Axiom/Infinity.v
@@ -1,0 +1,41 @@
+Require Import Coq.Lists.List.
+Require Import Coq.Strings.String.
+
+Require Import ZF.Meta.Env.
+Require Import ZF.Meta.Syntax.
+Require Import ZF.Meta.Term.Decl.
+Require Import ZF.Meta.Ty.
+
+Import ListNotations.
+
+Require Import ZF.Meta.Decl.Set.Empty.
+Require Import ZF.Meta.Decl.Set.Single.
+Require Import ZF.Meta.Decl.Set.Union2.
+
+(* exists a, empty :< a /\ forall x, x :< a -> union2 x (single x) :< a         *)
+Definition Infinity : DeclT :=
+  {| paraT := []
+  ;  resT  := TyProp
+  ;  bodyT :=
+      Ex VarTySet
+        (And
+          (Elem (IdentT "empty" []) (Var 0))
+          (All VarTySet
+            (Imp
+              (Elem (Var 0) (Var 1))
+              (Elem
+                (IdentT "union2" [Var 0; IdentT "single" [Var 0]])
+                (Var 1)))))
+  |}.
+
+Definition imports : Env := Env.unions
+  [ Empty.exports
+  ; Single.exports
+  ; Union2.exports
+  ].
+
+Definition exports : Env := Env.fromListT
+  [ ("Infinity"%string, Infinity)
+  ].
+
+Definition env : Env := Env.union imports exports.
