coq/ZF/Meta/Decl/Set/Single.v
@@ -1,0 +1,23 @@
+Require Import Coq.Lists.List.
+Require Import Coq.Strings.String.
+
+Require Import ZF.Meta.Env.
+Require Import ZF.Meta.Syntax.
+Require Import ZF.Meta.Term.Decl.
+Require Import ZF.Meta.Ty.
+
+Import ListNotations.
+
+Definition single : DeclT :=
+  {| paraT := [TySet]
+  ;  resT  := TySet
+  ;  bodyT := HoleT TySet
+  |}.
+
+Definition imports : Env := Env.empty.
+
+Definition exports : Env := Env.fromListT
+  [ ("single"%string, single)
+  ].
+
+Definition env : Env := Env.union imports exports.
